make progress on defining fixpoints

theories/rust_typing/fixpoint.v
@@ -1,11 +1,11 @@
 From refinedrust Require Import type.
 From iris.prelude Require Import options.
 
-Section fixpoint_def.
+Section type_inh. 
   Context `{!typeGS Σ}.
 
   (* We need [Inhabited T_rt] because of [ty_rt_inhabited]. *)
-  Context {T_rt : Type} `{!Inhabited T_rt} (T : type T_rt → type T_rt) {HT : TypeContractive T}.
+  Context {T_rt : Type} `{!Inhabited T_rt}.
 
   Global Program Instance simple_type_inhabited : Inhabited (simple_type T_rt) := populate {|
       st_own π r v := ⌜v = []⌝%I;
@@ -29,24 +29,355 @@ Section fixpoint_def.
     destruct mt; simpl; iPureIntro; done.
   Qed.
   Global Instance type_inhabited : Inhabited (type T_rt) := populate (ty_of_st _ inhabitant).
+End type_inh.
 
-  Local Instance type_2_contractive : Contractive (Nat.iter 2 T).
-  Proof using Type*.
-    intros n ? **. simpl.
-    apply dist_later_S. apply type_dist2_dist_later. 
-    apply HT. 
-    apply HT. 
-    apply type_later_dist2_later.
-    done.
+Section fixpoint_def.
+  Context `{!typeGS Σ}.
+  
+  (* We assume a contractive functor *)
+  Context {rt : Type} (F : type rt → type rt) `{Hcr : !TypeContractive F}.
+  (* [rt] needs to be inhabited *)
+  Context `{!Inhabited rt}.
+
+  (* Iterate the functor [S n] times, starting with the inhabitant.
+     We use at least one iteration, so that the [ty_syn_type] is always constant.
+  *)
+  Definition Fn n := Nat.iter (S n) F inhabitant. 
+
+  Lemma Fn_syn_type_const n m : 
+    ty_syn_type (Fn n) = ty_syn_type (Fn m).
+  Proof using Hcr.
+    unfold Fn. simpl. apply Hcr.
+  Qed.
+  Lemma Fn_sidecond_const n m : 
+    ty_sidecond (Fn n) ≡ ty_sidecond (Fn m).
+  Proof using Hcr.
+    unfold Fn; simpl. eapply Hcr.
   Qed.
 
-  Definition type_fixpoint : type T_rt := fixpointK 2 T.
+  Search logical_step.
+
+
+  (* what can we prove about ghost_drop? *)
+  (* TODO The problem: 
+     I don't have laters over there. 
+     With the current setup, I probably cannot prove that it's a fixpoint wrt ghost_drop 
+
+     What do I expect the ghost_drop to be?
+
+     Let's say I have a linked list defined via Box.
+     I store mutable references in there.
+     Now I drop the linked list.
+     Ideally, I want a bigsep over all the observations.
+     - i.e., the Box needs to pass through the inner ghost drop, with the respective smaller refinement.
+      For this, I need to make this guarded over that also. 
+     I guess in the end I get some laters. But I can also provide some later credits. 
+     Ideally, logical_step would be contractive....
+     But I guess it's not.
+
+     I want amortized reasoning also at the logic level!! 
+
+     Alternatively, I would define a version that has laters and provides a later credit, to make it guarded.
+     Then I want to derive something on top that uses the logical step.
+
+   *)
+
+  Lemma Fn_lfts_const n m : 
+    ty_lfts (Fn n) = ty_lfts (Fn m).
+  Proof.
+    (* TODO *)
+    (*
+       What can I do about this? 
+       - we need a notion of lifetime equivalence that is okay with idempotence.
+       - 
+
+
+
+    *)
+
+
+  Admitted.
+
+
+  Lemma Fn_has_op_type_const n m ot mt :
+    ty_has_op_type (Fn n) ot mt ↔ ty_has_op_type (Fn m) ot mt.
+  Proof using Hcr.
+    unfold Fn; simpl. eapply Hcr.
+  Qed.
+
+  Lemma Fn_succ n : 
+    Fn (S n) = F (Fn n).
+  Proof. done. Qed.
+
+  (* We define a chain consisting of the ownership and sharing predicate and take the fixpoint over that. *)
+  Definition ty_own_shrO : ofe := prodO (thread_id -d> rt -d> val -d> iPropO Σ) (lft -d> thread_id -d> rt -d> loc -d> iPropO Σ).
+
+  (* We have the [2+] in order to fix up the [0] base case *)
+  Lemma ty_own_shr_cauchy (i n : nat) : 
+    n ≤ i →
+    (∀ π r v, dist_later n (v ◁ᵥ{π} r @ (Fn (2+i)))%I (v ◁ᵥ{π} r @ (Fn (2+n)))%I) ∧
+    (∀ κ π r l, (l ◁ₗ{π, κ} r @ (Fn (2+i)))%I ≡{n}≡ (l ◁ₗ{π, κ} r @ (Fn (2+n)))%I).
+  Proof using Hcr.
+    induction n as [ | n IH] in i |-*; simpl; intros Hle.
+    { split; first (intros; dist_later_intro; lia).
+      intros. eapply Hcr.
+      - eapply Hcr.
+      - eapply Hcr.
+      - intros. dist_later_2_intro; lia.
+      - intros. dist_later_intro; lia.
+    } 
+    destruct i; first lia.
+    destruct (IH i) as [Hown Hshr]; first lia.
+    split.
+    - intros. dist_later_intro.
+      simpl. eapply Hcr.
+      + eapply Hcr.
+      + eapply Hcr.
+      + intros. dist_later_intro.
+        eapply dist_later_lt; [eapply Hown | ]. lia.
+      + intros. eapply dist_le; first apply Hshr. lia.
+    - intros. simpl. eapply Hcr.
+      + eapply Hcr.
+      + eapply Hcr.
+      + intros. dist_later_2_intro. eapply dist_later_lt; first done. lia. 
+      + intros. dist_later_intro. eapply dist_le; first apply Hshr. lia.
+  Qed.
+
+  (* [3+] because that's what we need to apply the above lemma proving that the chain is Cauchy *)
+  Program Definition F_ty_own_val_ty_shr_chain : chain ty_own_shrO := {|
+    chain_car n := ((Fn (3 + n)).(ty_own_val), (Fn (3+n)).(ty_shr))
+  |}.
+  Next Obligation.
+    simpl. intros n i Hle.
+    destruct (ty_own_shr_cauchy (S i) (S n)) as [Hown Hshr]; first lia.
+    constructor; simpl.
+    - intros ???. eapply dist_later_lt; first eapply Hown. lia.
+    - intros ????. eapply dist_le; first eapply Hshr. lia.
+  Qed.
+  Definition F_ty_own_val_ty_shr_fixpoint : ty_own_shrO :=
+    compl F_ty_own_val_ty_shr_chain.
+
+  (* Now we are ready to define the fixpoint *)
+  (* For the ownership and sharing predicate, we take the fixpoint found above. *)
+  (* For the other components, we use the 0 base case (where the functor is applied at least once) in order to be able to show the unfolding equation later. *)
+  Program Definition type_fixpoint : type rt := {|
+    ty_rt_inhabited := _;
+    ty_syn_type := (Fn 0).(ty_syn_type);
+    _ty_has_op_type := (Fn 0).(_ty_has_op_type _);
+    ty_own_val := F_ty_own_val_ty_shr_fixpoint.1;
+    ty_shr := F_ty_own_val_ty_shr_fixpoint.2;
+    ty_sidecond := (Fn 0).(ty_sidecond);
+    ty_ghost_drop := (Fn 0).(ty_ghost_drop);
+    ty_lfts := (Fn 0).(ty_lfts);
+    ty_wf_E := (Fn 0).(ty_wf_E);
+  |}.
+  Next Obligation.
+    intros. unfold F_ty_own_val_ty_shr_fixpoint.
+    eapply @limit_preserving.
+    - eapply bi.limit_preserving_entails; first apply _.
+      intros ? [] [] Heq. f_equiv. eapply Heq.
+    - intros ?. 
+      simpl. erewrite Fn_syn_type_const. eapply ty_has_layout.
+  Qed.
+  Next Obligation.
+    eapply _ty_op_type_stable.
+  Qed.
+  Next Obligation.
+    intros. unfold F_ty_own_val_ty_shr_fixpoint.
+    eapply @limit_preserving.
+    - eapply bi.limit_preserving_entails; first apply _.
+      intros ? [] [] Heq. f_equiv. eapply Heq.
+    - intros ?. 
+      simpl. erewrite Fn_sidecond_const. eapply ty_own_val_sidecond.
+  Qed.
+  Next Obligation.
+    intros. unfold F_ty_own_val_ty_shr_fixpoint.
+    eapply @limit_preserving.
+    - eapply bi.limit_preserving_entails; first apply _.
+      intros ? [] [] Heq. f_equiv. eapply Heq.
+    - intros ?. 
+      simpl. erewrite Fn_sidecond_const. eapply ty_shr_sidecond.
+  Qed.
+  Next Obligation.
+    intros. unfold F_ty_own_val_ty_shr_fixpoint.
+    eapply @limit_preserving.
+    - eapply bi.limit_preserving_Persistent.
+      intros ? [] [] Heq. eapply Heq.
+    - intros ?. 
+      simpl. eapply ty_shr_persistent.
+  Qed.
+  Next Obligation.
+    intros. unfold F_ty_own_val_ty_shr_fixpoint.
+    eapply @limit_preserving.
+    - eapply bi.limit_preserving_entails; first apply _.
+      intros ? [] [] Heq. f_equiv. eapply Heq.
+    - intros ?. 
+      simpl. erewrite Fn_syn_type_const. eapply ty_shr_aligned.
+  Qed.
+  Next Obligation.
+    intros. unfold F_ty_own_val_ty_shr_fixpoint.
+    eapply @limit_preserving.
+    - eapply bi.limit_preserving_entails; first apply _.
+      intros ? [] [] Heq. do 8 f_equiv. 
+      { do 2 f_equiv. apply Heq. }
+      apply Heq.
+    - intros ?. simpl. 
+      erewrite Fn_syn_type_const. 
+      erewrite Fn_lfts_const.
+      eapply ty_share.
+      done.
+  Qed.
+  Next Obligation.
+    intros. unfold F_ty_own_val_ty_shr_fixpoint.
+    eapply @limit_preserving.
+    - eapply bi.limit_preserving_entails; first apply _.
+      intros ? [] [] Heq. do 2 f_equiv; eapply Heq.
+    - intros ?. 
+      simpl. eapply ty_shr_mono.
+  Qed.
+  Next Obligation.
+    intros. unfold F_ty_own_val_ty_shr_fixpoint.
+    eapply @limit_preserving.
+    - eapply bi.limit_preserving_entails; first apply _.
+      intros ? [] [] Heq. f_equiv. eapply Heq.
+    - intros ?. simpl.
+
+      (* TODO *)
+  Admitted.
+  Next Obligation.
+    intros. unfold F_ty_own_val_ty_shr_fixpoint.
+    eapply @limit_preserving.
+    - eapply bi.limit_preserving_entails; first apply _.
+      intros ? [] [] Heq. f_equiv; first eapply Heq.
+      f_equiv. eapply Heq.
+    - intros ?. 
+      simpl. eapply _ty_memcast_compat.
+      rewrite -ty_has_op_type_unfold.
+      eapply Fn_has_op_type_const. by rewrite ty_has_op_type_unfold. 
+  Qed.
+
+  Lemma type_fixpoint_own_val_unfold_n n v π r : 
+    (v ◁ᵥ{π} r @ type_fixpoint)%I ≡{n}≡ (v ◁ᵥ{π} r @ Fn (3+n))%I.
+  Proof.
+    rewrite {1}/ty_own_val/=/F_ty_own_val_ty_shr_fixpoint/=.
+    etrans. { apply (conv_compl n _). }
+    simpl. done.
+  Qed.
+  Lemma type_fixpoint_shr_unfold_n n l κ π r : 
+    (l ◁ₗ{π, κ} r @ type_fixpoint)%I ≡{n}≡ (l ◁ₗ{π, κ} r @ Fn (3+n))%I.
+  Proof.
+    rewrite {1}/ty_shr/=/F_ty_own_val_ty_shr_fixpoint/=.
+    etrans. { apply (conv_compl n _). }
+    simpl. done.
+  Qed.
+
+  Lemma type_fixpoint_syn_type : 
+    type_fixpoint.(ty_syn_type) = (Fn 0).(ty_syn_type).
+  Proof. done. Qed.
+  Lemma type_fixpoint_sidecond :
+    type_fixpoint.(ty_sidecond) = (Fn 0).(ty_sidecond).
+  Proof. done. Qed.
+
+  Lemma type_fixpoint_own_val_unfold v π r : 
+    (v ◁ᵥ{π} r @ type_fixpoint)%I ≡ (v ◁ᵥ{π} r @ F type_fixpoint)%I.
+  Proof.
+    apply equiv_dist => n. rewrite type_fixpoint_own_val_unfold_n.
+    rewrite Fn_succ.
+    eapply Hcr.
+    - rewrite type_fixpoint_syn_type. erewrite Fn_syn_type_const; done.
+    - rewrite type_fixpoint_sidecond. erewrite Fn_sidecond_const; done.
+    - intros. dist_later_intro.
+      rewrite type_fixpoint_own_val_unfold_n.
+      eapply dist_later_lt.
+      { eapply (ty_own_shr_cauchy n (S m)). lia. }
+      lia.
+    - intros.
+      rewrite type_fixpoint_shr_unfold_n.
+      etrans. 
+      { symmetry. eapply (ty_own_shr_cauchy (S n) (n)). lia. }
+      done.
+  Qed.
+  Lemma type_fixpoint_shr_unfold l π κ r : 
+    (l ◁ₗ{π, κ} r @ type_fixpoint)%I ≡ (l ◁ₗ{π, κ} r @ F type_fixpoint)%I.
+  Proof.
+    apply equiv_dist => n. rewrite type_fixpoint_shr_unfold_n.
+    rewrite Fn_succ.
+    eapply Hcr.
+    - rewrite type_fixpoint_syn_type. erewrite Fn_syn_type_const; done.
+    - rewrite type_fixpoint_sidecond. erewrite Fn_sidecond_const; done.
+    - intros. dist_later_2_intro.
+      rewrite type_fixpoint_own_val_unfold_n.
+      simpl. eapply dist_later_lt.
+      { eapply (ty_own_shr_cauchy n). lia. }
+      lia.
+    - intros. dist_later_intro.
+      rewrite type_fixpoint_shr_unfold_n.
+      eapply dist_le.
+      { eapply (ty_own_shr_cauchy n (S m) ). lia. }
+      lia. 
+  Qed.
+  Lemma type_fixpoint_equiv : 
+    type_fixpoint ≡ F type_fixpoint.
+  Proof.
+    (* The fixpoint operator does NOT preserve everything (e.g. the inhabitant),
+       so this does not hold. *)
+  Abort.
+
+  Lemma type_fixpoint_ty_lfts : 
+    type_fixpoint.(ty_lfts) = (Fn 0).(ty_lfts).
+  Proof.
+  Admitted.
+  Lemma type_fixpoint_ty_wf_E : 
+    type_fixpoint.(ty_wf_E) = (Fn 0).(ty_wf_E).
+  Proof.
+  Admitted.
+
+  (*Lemma type_fixpoint_ghost_drop : *)
+    (*type_fixpoint.(ty_ghost_drop) *)
+
 End fixpoint_def.
 
 Lemma type_fixpoint_ne `{!typeGS Σ} {rt} `{!Inhabited rt} (T1 T2 : type rt → type rt)
-    `{!TypeContractive T1, !TypeContractive T2} n :
+    `{!TypeContractive T1, !TypeContractive T2, !NonExpansive T2} n :
   (∀ t, T1 t ≡{n}≡ T2 t) → type_fixpoint T1 ≡{n}≡ type_fixpoint T2.
-Proof. eapply fixpointK_ne; apply type_contractive_ne, _. Qed.
+Proof. 
+  intros Heq.
+  constructor.
+  - done.
+  - simpl.
+    destruct (Heq inhabitant) as [_ Hot].
+    move: Hot. rewrite ty_has_op_type_unfold. done.
+  - iIntros (???).
+    rewrite !type_fixpoint_own_val_unfold_n.
+    f_equiv. 
+    generalize (3+n) as m.
+    induction m as [ | m IH]; simpl.
+    { apply Heq. }
+    specialize (Heq (Fn T1 m)).
+    setoid_rewrite Heq. 
+    (* here we need that T2 is also non-expansive *)
+    by rewrite IH.
+  - iIntros (????). 
+    rewrite !type_fixpoint_shr_unfold_n.
+    f_equiv. 
+    generalize (3+n) as m.
+    induction m as [ | m IH]; simpl.
+    { apply Heq. }
+    specialize (Heq (Fn T1 m)).
+    setoid_rewrite Heq. 
+    (* here we need that T2 is also non-expansive *)
+    by rewrite IH.
+  - simpl. destruct (Heq inhabitant). done.
+  - simpl. destruct (Heq inhabitant). done.
+  - intros. simpl. destruct (Heq inhabitant). done.
+  - intros. simpl. destruct (Heq inhabitant). done.
+  - intros. simpl. destruct (Heq inhabitant). done.
+Qed.
+
+(* TODO: should we also have something that states that fixpoint is TypeNonExpansive / TypeContractive? *)
+(*Lemma type_fixpoint_type_ne `{!typeGS Σ} {rt} `{!Inhabited rt} (T1 T2 : type rt → type rt)*)
+    (*`{!TypeContractive T1, !TypeContractive T2, !NonExpansive T2} n :*)
+  (*(∀ t, T1 t ≡{n}≡ T2 t) → TypeNonExpansive (λ type_fixpoint T1)*)
 
 Section fixpoint.
   Context `{!typeGS Σ}.
@@ -55,22 +386,27 @@ Section fixpoint.
   Global Instance type_fixpoint_copy :
     (∀ `(!Copyable ty), Copyable (T ty)) → Copyable (type_fixpoint T).
   Proof.
-    intros ?. unfold type_fixpoint. apply fixpointK_ind.
-    - apply type_contractive_ne, _.
-    - apply copy_equiv.
-    - exists inhabitant. apply _.
-    - done.
-    - (* If Copy was an Iris assertion, this would be trivial -- we'd just
-         use limit_preserving_and directly. However, on the Coq side, it is
-         more convenient as a record -- so this is where we pay. *)
-      eapply (limit_preserving_ext (λ _, _ ∧ _)).
-      { split; (intros [H1 H2]; split; [apply H1|apply H2]). }
-      apply limit_preserving_and; repeat (apply limit_preserving_forall=> ?).
-      { apply bi.limit_preserving_Persistent; solve_proper. }
-      apply limit_preserving_impl'. 
-      { intros ?? [? ??? ->]. done. }
-      apply limit_preserving_impl', bi.limit_preserving_emp_valid;
-        solve_proper_core ltac:(fun _ => eapply ty_size_ne || f_equiv).
+    intros ?.
+    (* the chain is copyable *)
+    assert (∀ n, Copyable (Fn T n)). 
+    { induction n as [ | n IH]; simpl; apply _. }
+    constructor.
+    - intros. rewrite /ty_own_val/= /F_ty_own_val_ty_shr_fixpoint/=.
+      eapply @limit_preserving.
+      { eapply bi.limit_preserving_Persistent. 
+        intros n [][][Heq1 Heq2].
+        simpl in *. apply Heq1. }
+      apply _.
+    - intros ? ? ? ? ? ? ? ? ? Hst. intros. 
+      rewrite /ty_shr/ty_own_val/= /F_ty_own_val_ty_shr_fixpoint/=.
+      eapply @limit_preserving.
+      { eapply bi.limit_preserving_entails; first apply _. 
+        intros n [][][Heq1 Heq2].
+        repeat f_equiv; simpl; [apply Heq2 | apply Heq1]. }
+      intros ?. 
+      eapply copy_shr_acc; [done | | done].
+      move: Hst. rewrite type_fixpoint_syn_type.  
+      erewrite Fn_syn_type_const; done.
   Qed.
 
   (*
@@ -99,19 +435,38 @@ Section fixpoint.
   Qed.
   *)
 
-  Lemma type_fixpoint_unfold : type_fixpoint T ≡ T (type_fixpoint T).
-  Proof. apply fixpointK_unfold. by apply type_contractive_ne. Qed.
-
-  Lemma fixpoint_unfold_eqtype E L r : eqtype E L r r (type_fixpoint T) (T (type_fixpoint T)).
+  Lemma type_fixpoint_incl_1 r : ⊢ type_incl r r (type_fixpoint T) (T (type_fixpoint T)).
   Proof. 
-    apply eqtype_unfold.
-    iIntros (?) "HL HE".
-    iSplitR; last iSplitR; last iSplitR.
-    - iPureIntro. by rewrite {1}type_fixpoint_unfold.
-    - rewrite {1}type_fixpoint_unfold. eauto.
-    - iModIntro. iIntros (??).
-      rewrite {1}type_fixpoint_unfold. eauto.
-    - iModIntro. iIntros (???).
-      rewrite {1}type_fixpoint_unfold. eauto.
+    iSplit; last iSplit; last iSplit.
+    - iPureIntro. rewrite !type_fixpoint_syn_type. apply HT.
+    - iModIntro. simpl. rewrite type_ctr_sidecond. eauto.
+    - iModIntro. iIntros (π v). rewrite type_fixpoint_own_val_unfold. eauto.
+    - iModIntro. iIntros (???). rewrite type_fixpoint_shr_unfold. eauto.
   Qed.
+  Lemma type_fixpoint_incl_2 r : ⊢ type_incl r r (T (type_fixpoint T)) (type_fixpoint T).
+  Proof. 
+    iSplit; last iSplit; last iSplit.
+    - iPureIntro. rewrite !type_fixpoint_syn_type. apply HT.
+    - iModIntro. simpl. rewrite type_ctr_sidecond. eauto.
+    - iModIntro. iIntros (π v). rewrite type_fixpoint_own_val_unfold. eauto.
+    - iModIntro. iIntros (???). rewrite type_fixpoint_shr_unfold. eauto.
+  Qed.
+
+  Lemma type_fixpoint_subtype_1 E L r : subtype E L r r (type_fixpoint T) (T (type_fixpoint T)).
+  Proof. 
+    iIntros (?) "HL HE". iApply type_fixpoint_incl_1.
+  Qed.
+  Lemma type_fixpoint_subtype_2 E L r : subtype E L r r (T (type_fixpoint T)) (type_fixpoint T).
+  Proof. 
+    iIntros (?) "HL HE". iApply type_fixpoint_incl_2.
+  Qed.
+
+  Lemma type_fixpoint_unfold_eqtype E L r : eqtype E L r r (type_fixpoint T) (T (type_fixpoint T)).
+  Proof. 
+    split.
+    - apply type_fixpoint_subtype_1.
+    - apply type_fixpoint_subtype_2.
+  Qed.
+
+  (* TODO subtyping -- think of the right lemmas here *)
 End fixpoint.
